LeanYjs/IntegrateProof.lean
@@ -1564,23 +1564,28 @@ lemma findPtrIdx_lt_size_getElem {p : YjsPtr A} :
     subst p
     simp
 
-structure InsertOk (arr : Array (YjsItem A)) (newItem : YjsItem A) where
-  origin_lt_rightOrigin : YjsLt' (A := A) newItem.origin newItem.rightOrigin
+structure IsItemValid (item : YjsItem A) where
+  origin_lt_rightOrigin : YjsLt' (A := A) item.origin item.rightOrigin
   reachable_YjsLeq' : (∀ (x : YjsPtr A),
-      OriginReachable (YjsPtr.itemPtr newItem) x →
-      YjsLeq' (A := A) x newItem.origin ∨ YjsLeq' (A := A) newItem.rightOrigin x)
+      OriginReachable (YjsPtr.itemPtr item) x →
+      YjsLeq' (A := A) x item.origin ∨ YjsLeq' (A := A) item.rightOrigin x)
+
+abbrev YjsItem.isValid : YjsItem A → Prop := IsItemValid
+
+structure InsertOk (arr : Array (YjsItem A)) (newItem : YjsItem A) where
   id_eq_YjsLeq' : ∀ (x : YjsItem A),
     ArrSet arr.toList (YjsPtr.itemPtr x) →
     x.id.clientId = newItem.id.clientId → x.id.clock < newItem.id.clock
 
 theorem YjsArrInvariant_integrate (newItem : YjsItem A) (arr newArr : Array (YjsItem A)) :
   YjsArrInvariant arr.toList
+  → newItem.isValid
   -> InsertOk arr newItem
   -> integrate newItem arr = Except.ok newArr
   -> ∃ i ≤ arr.size, newArr = arr.insertIdxIfInBounds i newItem ∧ YjsArrInvariant newArr.toList := by
-  intros harrinv h_InsertOk hintegrate
-  obtain ⟨ horigin_consistent, hreachable_consistent, hsameid_consistent ⟩ :=
-    h_InsertOk
+  intros harrinv h_valid h_InsertOk hintegrate
+  obtain ⟨ hsameid_consistent ⟩ := h_InsertOk
+  obtain ⟨ horigin_consistent, hreachable_consistent ⟩ := h_valid
   unfold integrate at hintegrate
   generalize heqleft : findPtrIdx newItem.origin arr = leftIdx at hintegrate
   obtain ⟨ _ ⟩ | ⟨ leftIdx ⟩ := leftIdx; cases hintegrate
@@ -1620,7 +1625,7 @@ theorem YjsArrInvariant_integrate (newItem : YjsItem A) (arr newArr : Array (Yjs
     apply findPtrIdx_ge_minus_1 at heqleft
     omega
 
-  simp at hintegrate
+  simp [findIntegratedIndex] at hintegrate
 
   generalize hloop :
    forIn (m := Except IntegrateError) (ρ := List ℕ) (α := ℕ) (β := MProd ℤ Bool) (List.range' 1 ((rightIdx - leftIdx).toNat - 1) 1) ⟨leftIdx + 1, false⟩ (fun offset r => do
@@ -1877,8 +1882,8 @@ theorem insertOk_mono (arr1 arr2 : Array (YjsItem A)) (x : YjsItem A) :
   -> InsertOk arr1 x
   -> InsertOk arr2 x := by
   intros harrinv1 harrinv2 h_arr1_subset_arr2 h_id_neq h_InsertOk
-  obtain ⟨ horigin_consistent, hreachable_consistent, hsameid_consistent ⟩ := h_InsertOk
-  constructor <;> try assumption
+  obtain ⟨ hsameid_consistent ⟩ := h_InsertOk
+  constructor; try assumption
   . intros y hy_in_arr2 hid_eq
     have hy_in_arr1 : ArrSet arr1.toList y := by
       simp [ArrSet]
@@ -1929,9 +1934,11 @@ theorem insertIdxIfInBounds_insertOk (arr : Array (YjsItem A)) (a x : YjsItem A)
       contradiction
   . assumption
 
-theorem integrate_commutative (a b : YjsItem A) (arr1 arr2 arr3 arr2' arr3' : Array (YjsItem A)) :
+theorem integrate_ok_commutative (a b : YjsItem A) (arr1 arr2 arr3 arr2' arr3' : Array (YjsItem A)) :
   YjsArrInvariant arr1.toList
   -> a.id.clientId ≠ b.id.clientId
+  → a.isValid
+  → b.isValid
   -> InsertOk arr1 a
   -> InsertOk arr1 b
   -> integrate a arr1 = Except.ok arr2
@@ -1939,10 +1946,11 @@ theorem integrate_commutative (a b : YjsItem A) (arr1 arr2 arr3 arr2' arr3' : Ar
   -> integrate b arr1 = Except.ok arr2'
   -> integrate a arr2' = Except.ok arr3'
   -> arr3 = arr3' := by
-  intros harrinv hcid_neq_bid h_InsertOk_a h_InsertOk_b hintegrate_a hintegrate_b hintegrate_b' hintegrate_a'
+  intros harrinv hcid_neq_bid h_a_valid h_b_valid h_InsertOk_a h_InsertOk_b hintegrate_a hintegrate_b hintegrate_b' hintegrate_a'
 
   have ⟨ idx2, h_idx2, arr2_insertIdx, arr2_inv ⟩ : ∃ idx ≤ arr1.size, arr2 = arr1.insertIdxIfInBounds idx a ∧ YjsArrInvariant arr2.toList := by
     apply YjsArrInvariant_integrate a arr1 arr2
+    assumption
     assumption
     assumption
     assumption
@@ -1953,6 +1961,7 @@ theorem integrate_commutative (a b : YjsItem A) (arr1 arr2 arr3 arr2' arr3' : Ar
 
   have ⟨ idx2', h_idx2', arr2'_insertIdx, arr2'_inv ⟩ : ∃ idx ≤ arr1.size, arr2' = arr1.insertIdxIfInBounds idx b ∧ YjsArrInvariant arr2'.toList := by
     apply YjsArrInvariant_integrate b arr1 arr2'
+    assumption
     assumption
     assumption
     assumption
@@ -1969,9 +1978,11 @@ theorem integrate_commutative (a b : YjsItem A) (arr1 arr2 arr3 arr2' arr3' : Ar
     assumption
     assumption
     assumption
+    assumption
 
   have ⟨ idx3', h_idx3', arr3'_insertIdx, arr3'_inv ⟩ : ∃ idx ≤ arr2'.size, arr3' = arr2'.insertIdxIfInBounds idx a ∧ YjsArrInvariant arr3'.toList := by
     apply YjsArrInvariant_integrate a arr2' arr3'
+    assumption
     assumption
     assumption
     assumption
@@ -1998,3 +2009,307 @@ theorem integrate_commutative (a b : YjsItem A) (arr1 arr2 arr3 arr2' arr3' : Ar
     rw [List.mem_insertIdx h_idx3, List.mem_insertIdx h_idx3', List.mem_insertIdx h_idx2, List.mem_insertIdx h_idx2']
     simp
     tauto
+
+theorem forIn_ok {α β : Type} {lst : List α} {init : β} {f : α → β → Except IntegrateError (ForInStep β)} :
+  (∀ x ∈ lst, ∀ state, ∃ state', f x state = Except.ok state')
+  → ∃ finalState, forIn lst init f = Except.ok finalState := by
+  intros h_f
+  induction lst generalizing init with
+  | nil =>
+    exists init
+  | cons x xs ih =>
+    simp
+    have ⟨ state', hfx ⟩ := h_f x (by simp) init
+    rw [hfx]
+    simp [bind, Except.bind]
+    cases state' with
+    | done finalState =>
+      exists finalState
+    | yield nextState =>
+      simp
+      replace ⟨ finalState, ih ⟩ := ih (init := nextState) (fun y hy state => h_f y (by simp [hy]) state)
+      use finalState
+
+theorem ArrSet_findPtrIdx_eq_some {p : YjsPtr A} {arr : Array (YjsItem A)} :
+  ArrSet arr.toList p
+  → ∃idx, findPtrIdx p arr = Except.ok idx:= by
+  intros h_arrset
+  cases p with
+  | first =>
+    exists -1
+  | last =>
+    exists arr.size
+  | itemPtr p =>
+    simp [findPtrIdx]
+    rw [Array.findIdx?_eq_some_of_exists]
+    simp; constructor; eq_refl
+    simp [ArrSet] at h_arrset
+    use p; simp; assumption
+
+theorem findIntegratedIndex_safe {leftIdx rightIdx : ℤ} {arr : Array (YjsItem A)} {newItem: YjsItem A} :
+  YjsArrInvariant arr.toList
+  → -1 ≤ leftIdx → leftIdx ≤ arr.size
+  → -1 ≤ rightIdx → rightIdx ≤ arr.size
+  → ∃ idx', findIntegratedIndex leftIdx rightIdx newItem arr = Except.ok idx' := by
+  intros harrinv hleft_ge hleft_le hright_ge hright_le
+  unfold findIntegratedIndex
+  simp
+
+  have ⟨ ⟨ dest, scanning ⟩, loop_ok ⟩ :
+    ∃ idx, forIn (m := Except IntegrateError) (ρ := List ℕ) (α := ℕ) (β := MProd ℤ Bool)
+      (List.range' 1 ((rightIdx - leftIdx).toNat - 1)) ⟨leftIdx + 1, false⟩ (fun offset r => do
+        let other ← getElemExcept arr (leftIdx + ↑offset).toNat
+        let oLeftIdx ← findPtrIdx other.origin arr
+        let oRightIdx ← findPtrIdx other.rightOrigin arr
+        if oLeftIdx < leftIdx then pure (ForInStep.done ⟨r.fst, r.snd⟩)
+          else
+            if oLeftIdx = leftIdx then
+              if other.id.clientId < newItem.id.clientId then
+                pure (ForInStep.yield ⟨max (leftIdx + ↑offset) 0 + 1, false⟩)
+              else
+                if oRightIdx = rightIdx then pure (ForInStep.done ⟨r.fst, r.snd⟩)
+                else pure (ForInStep.yield ⟨r.fst, true⟩)
+            else
+              if r.snd = false then pure (ForInStep.yield ⟨max (leftIdx + ↑offset) 0 + 1, r.snd⟩)
+              else pure (ForInStep.yield ⟨r.fst, r.snd⟩)) = Except.ok idx := by
+    apply forIn_ok
+    intros offset h_offset_mem state
+    obtain ⟨ destIdx, scanning ⟩ := state
+
+    simp at h_offset_mem
+
+    have ⟨ other, h_other_eq ⟩ : ∃ other, arr[(leftIdx + ↑offset).toNat]? = some other := by
+      rw [Array.getElem?_eq_getElem (by omega)]
+      simp
+
+    have h_other_ok : getElemExcept arr (leftIdx + ↑offset).toNat = Except.ok other := by
+      simp [getElemExcept]
+      rw [h_other_eq]
+      simp; eq_refl
+
+    rw [h_other_ok, ok_bind]
+
+    have ArrSet_other_origin : ArrSet arr.toList other.origin := by
+      obtain ⟨ o, r, id, c ⟩ := other
+      apply harrinv.closed.closedLeft o r id c
+      simp [ArrSet]
+      rw [getElem?_eq_some_iff] at h_other_eq
+      obtain ⟨ _, h_other_eq ⟩ := h_other_eq
+      rw [<-h_other_eq]
+      simp
+
+    have ArrSet_other_rightOrigin : ArrSet arr.toList other.rightOrigin := by
+      obtain ⟨ o, r, id, c ⟩ := other
+      apply harrinv.closed.closedRight o r id c
+      simp [ArrSet]
+      rw [getElem?_eq_some_iff] at h_other_eq
+      obtain ⟨ _, h_other_eq ⟩ := h_other_eq
+      rw [<-h_other_eq]
+      simp
+
+    have ⟨ oLeftIdx, h_oLeftIdx_ok ⟩ : ∃ oLeftIdx, findPtrIdx other.origin arr = Except.ok oLeftIdx := by
+      simp [getElemExcept] at h_other_ok
+      apply ArrSet_findPtrIdx_eq_some ArrSet_other_origin
+
+    rw [h_oLeftIdx_ok, ok_bind]
+
+    have ⟨ oRightIdx, h_oRightIdx_ok ⟩ : ∃ oRightIdx, findPtrIdx other.rightOrigin arr = Except.ok oRightIdx := by
+      simp [getElemExcept] at h_other_ok
+      apply ArrSet_findPtrIdx_eq_some ArrSet_other_rightOrigin
+
+    rw [h_oRightIdx_ok, ok_bind]
+
+    (repeat' (split)) <;> (constructor; eq_refl)
+
+  use dest.toNat; rw [loop_ok]
+  eq_refl
+
+theorem integrate_insert_eq_none {arr : Array (YjsItem A)} {newItem other: YjsItem A} :
+  YjsArrInvariant arr.toList
+  → InsertOk arr newItem
+  → ¬OriginReachable newItem (YjsPtr.itemPtr other)
+  → integrate newItem arr = Except.error e
+  → ∃ e', integrate newItem (arr.insertIdxIfInBounds idx other) = Except.error e' := by
+  intros harrinv h_InsertOk h_not_reachable hintegrate
+  unfold integrate at *
+
+  have h_neq_other_error : ∀ (t : YjsItem A), t ≠ other
+    → findPtrIdx t arr = Except.error e
+    → findPtrIdx t (arr.insertIdxIfInBounds idx other) = Except.error e := by
+    intros t heq h_neq_other
+    clear hintegrate
+    simp [findPtrIdx] at *
+    cases h_findPtrIdx_arr : Array.findIdx? (fun i => decide (i = t)) arr with
+    | some idx' =>
+      rw [h_findPtrIdx_arr] at h_neq_other; contradiction
+    | none =>
+      rw [h_findPtrIdx_arr] at h_neq_other; cases h_neq_other
+      cases heq' : Array.findIdx? (fun i => decide (i = t)) (arr.insertIdxIfInBounds idx other) with
+      | none =>
+        simp
+      | some idx' =>
+        have h_not_mem : t ∉ arr := by
+          intros hmem
+          rw [Array.findIdx?_eq_none_iff] at h_findPtrIdx_arr
+          simp at h_findPtrIdx_arr
+          apply h_findPtrIdx_arr _ hmem
+          simp
+        have h_mem : t ∈ arr.insertIdxIfInBounds idx other := by
+          rw [Array.findIdx?_eq_some_iff_getElem] at heq'
+          obtain ⟨ hlt, h1, _ ⟩ := heq'
+          simp at h1
+          subst t
+          simp
+        simp [Array.insertIdxIfInBounds] at h_mem
+        split at h_mem
+        . rw [Array.mem_insertIdx] at h_mem
+          cases h_mem with
+          | inl heq =>
+            contradiction
+          | inr hmem =>
+            contradiction
+        . contradiction
+
+  cases heqleft : findPtrIdx newItem.origin arr with
+  | error e =>
+    rw [heqleft] at hintegrate
+    cases hintegrate
+    have heqleft' : findPtrIdx newItem.origin (arr.insertIdxIfInBounds idx other) = Except.error e := by
+      cases h_origin_eq : newItem.origin with
+      | first =>
+        rw [h_origin_eq] at heqleft
+        simp [findPtrIdx] at heqleft
+        contradiction
+      | last =>
+        rw [h_origin_eq] at heqleft
+        simp [findPtrIdx] at heqleft
+        contradiction
+      | itemPtr p =>
+        rw [h_origin_eq] at heqleft
+        apply h_neq_other_error _ _ heqleft
+        intros heq
+        rw [<-heq, <-h_origin_eq] at h_not_reachable
+        apply h_not_reachable
+        obtain ⟨ o, r, id, c ⟩ := newItem
+        apply OriginReachable.reachable_single
+        apply OriginReachableStep.reachable
+    rw [heqleft']
+    exists e
+  | ok leftIdx =>
+    rw [heqleft, ok_bind] at hintegrate
+    cases heqleft' : findPtrIdx newItem.origin (arr.insertIdxIfInBounds idx other) with
+    | error e =>
+      simp [bind, Except.bind]
+      apply Nonempty.intro IntegrateError.notFound
+    | ok leftIdx' =>
+      rw [ok_bind]
+      cases heqright : findPtrIdx newItem.rightOrigin arr with
+      | error e =>
+        rw [heqright] at hintegrate
+        cases hintegrate
+        have heqright' : findPtrIdx newItem.rightOrigin (arr.insertIdxIfInBounds idx other) = Except.error e := by
+          cases h_rightOrigin_eq : newItem.rightOrigin with
+          | first =>
+            rw [h_rightOrigin_eq] at heqright
+            simp [findPtrIdx] at heqright
+            contradiction
+          | last =>
+            rw [h_rightOrigin_eq] at heqright
+            simp [findPtrIdx] at heqright
+            contradiction
+          | itemPtr p =>
+            rw [h_rightOrigin_eq] at heqright
+            apply h_neq_other_error _ _ heqright
+            intros heq
+            rw [<-heq, <-h_rightOrigin_eq] at h_not_reachable
+            apply h_not_reachable
+            obtain ⟨ o, r, id, c ⟩ := newItem
+            apply OriginReachable.reachable_single
+            apply OriginReachableStep.reachable_right
+        rw [heqright']
+        exists e
+      | ok rightIdx =>
+        rw [heqright, ok_bind] at hintegrate
+        have ⟨ destIdx, h_destIdx ⟩ : ∃ destdx, findIntegratedIndex leftIdx rightIdx newItem arr = Except.ok destdx := by
+          apply findIntegratedIndex_safe harrinv
+          apply findPtrIdx_ge_minus_1 at heqleft
+          assumption
+          apply findPtrIdx_le_size at heqleft
+          assumption
+          apply findPtrIdx_ge_minus_1 at heqright
+          assumption
+          apply findPtrIdx_le_size at heqright
+          assumption
+        rw [h_destIdx, ok_bind] at hintegrate
+        cases hintegrate
+
+theorem integrate_integrate_eq_none {arr : Array (YjsItem A)} {a b : YjsItem A} :
+  YjsArrInvariant arr.toList
+  → a.id.clientId ≠ b.id.clientId
+  → a.isValid
+  → b.isValid
+  → InsertOk arr a
+  → InsertOk arr b
+  → ¬OriginReachable a (YjsPtr.itemPtr b)
+  → integrate a arr = Except.error e
+  → integrate b arr = Except.ok arr2
+  → ∃ e', integrate a arr2 = Except.error e' := by
+  intros harrinv hcid_neq_bid h_a_valid h_b_valid h_InsertOk_a h_InsertOk_b h_not_reachable hintegrate_a
+  sorry
+
+theorem integrate_integrate_eq_some {arr : Array (YjsItem A)} {a b : YjsItem A} :
+  YjsArrInvariant arr.toList
+  → a.id.clientId ≠ b.id.clientId
+  → a.isValid
+  → b.isValid
+  → InsertOk arr a
+  → InsertOk arr b
+  → integrate a arr = Except.ok arr2
+  → integrate b arr = Except.ok arr2'
+  → ∃ arr3, integrate b arr2 = Except.ok arr3 := by
+  intros harrinv hcid_neq_bid h_a_valid h_b_valid h_InsertOk_a h_InsertOk_b h_not_reachable hintegrate_a
+  sorry
+
+theorem integrate_commutative (a b : YjsItem A) (arr1 : Array (YjsItem A)) :
+  YjsArrInvariant arr1.toList
+  -> a.id.clientId ≠ b.id.clientId
+  → ¬OriginReachable a (YjsPtr.itemPtr b)
+  → ¬OriginReachable b (YjsPtr.itemPtr a)
+  → a.isValid
+  → b.isValid
+  -> InsertOk arr1 a
+  -> InsertOk arr1 b
+  -> (do
+    let arr2 <- integrate a arr1;
+    integrate b arr2) =
+  (do
+    let arr2' <- integrate b arr1;
+    integrate a arr2') := by
+  intros harrinv hcid_neq_bid h_not_a_origin_b h_not_b_origin_a h_a_valid h_b_valid h_InsertOk_a h_InsertOk_b
+  cases h_eq_a : integrate a arr1 with
+  | error e_a =>
+    cases h_eq_b : integrate b arr1 with
+    | error e_b =>
+      simp [bind, Except.bind]
+    | ok arr2' =>
+      simp [bind, Except.bind]
+      have ⟨ e_a', h_integrate_a' ⟩ : ∃ e_a', integrate a arr2' = Except.error e_a' := by
+        apply integrate_integrate_eq_none harrinv hcid_neq_bid h_a_valid h_b_valid h_InsertOk_a h_InsertOk_b h_not_a_origin_b h_eq_a h_eq_b
+      rw [h_integrate_a']
+  | ok arr2 =>
+    cases h_eq_b : integrate b arr1 with
+    | error e_b =>
+      simp [bind, Except.bind]
+      have ⟨ e_b', h_integrate_b' ⟩ : ∃ e_b', integrate b arr2 = Except.error e_b' := by
+        apply integrate_integrate_eq_none harrinv _ h_b_valid h_a_valid h_InsertOk_b h_InsertOk_a h_not_b_origin_a h_eq_b h_eq_a
+        intros heq; rw [heq] at hcid_neq_bid; contradiction
+      rw [h_integrate_b']
+    | ok arr2' =>
+      simp [bind, Except.bind]
+      have ⟨ arr3', h_integrate_comm ⟩ : ∃ arr3', integrate a arr2' = Except.ok arr3' := by
+        apply integrate_integrate_eq_some harrinv _ h_b_valid h_a_valid h_InsertOk_b h_InsertOk_a h_eq_b h_eq_a
+        intros heq; rw [heq] at hcid_neq_bid; contradiction
+      have ⟨ arr3, h_integrate_comm' ⟩ : ∃ arr3, integrate b arr2 = Except.ok arr3 := by
+        apply integrate_integrate_eq_some harrinv hcid_neq_bid h_a_valid h_b_valid h_InsertOk_a h_InsertOk_b h_eq_a h_eq_b
+      rw [h_integrate_comm, h_integrate_comm']
+      rw [integrate_ok_commutative a b arr1 arr2 arr3 arr2' arr3' harrinv hcid_neq_bid h_a_valid h_b_valid h_InsertOk_a h_InsertOk_b h_eq_a h_integrate_comm' h_eq_b h_integrate_comm]
